Taskin/detProds.thy
@@ -7,176 +7,85 @@ text
  \<open>(A,w)\<close>. In this case we could replace every occurrence of \<open>A\<close> with \<open>w\<close> on the right-hand sides of the productions and the 
  language of the grammar would be preserved\<close>
 
-(* CFG? *)
-lemma Nts_un: 
-  "Nt ` Nts (a \<union> as) = Nt ` (Nts a) \<union> Nt ` (Nts as)"
-  unfolding Nts_def by blast
-
-(* CFG? *)
-lemma Tms_un: 
-  "Tm ` Tms (a \<union> as) = Tm ` (Tms a) \<union> Tm ` (Tms as)"
-  unfolding Tms_def by blast
-
-(* CFG? *)
-lemma nt_tm: "Nt ` nts_syms u \<union> Tm ` tms_of_syms u = set u"
-unfolding nts_syms_def tms_of_syms_def by (auto simp:image_iff) (metis sym.exhaust)
-
-(* CFG? *)
-lemma lhss_eq: "lhss ((A,u) # ps) = lhss ((A,s) # ps)"
-  by (auto simp: Lhss_def)
-
-(* CFG? *)
-lemma Lhss_set: 
-  "B \<notin> Lhss P \<Longrightarrow> (B,v) \<notin> P"
-  by (auto simp: Lhss_def)
-
-(* CFG? *)
-lemma fresh_Lhss: "B \<notin> Nts P \<Longrightarrow> B \<notin> Lhss P"
-by (auto simp: Lhss_def Nts_def)
-
-(* CFG? *)
-lemma nts_syms_set1: "B \<notin> nts_syms u \<Longrightarrow> Nt B \<notin> set u"
-  by (simp add: nts_syms_def)
-
-(* CFG? *)
-lemma nts_syms_set2: "Nt B \<notin> set u \<Longrightarrow> B \<notin> nts_syms u"
-  by (simp add: nts_syms_def)
-
-(* CFG? *)
-lemma Nts_to_syms: "B \<in> Nts P \<Longrightarrow> Nt B \<in> Syms P"
-unfolding Nts_def Syms_def
-apply (auto split: prod.splits)
- apply blast
-using nts_syms_set2 by fastforce
-
-(* CFG? *)
-lemma syms_to_Nts: "Nt B \<in> Syms P \<Longrightarrow> B \<in> Nts P"
-unfolding Nts_def Syms_def
-apply (auto split: prod.splits)
- apply blast
-using nts_syms_set1 by fastforce
-
-(* CFG? *)
-lemma Nts_syms_equI: "B \<in> Nts P \<longleftrightarrow> Nt B \<in> Syms P"
-  using Nts_to_syms syms_to_Nts by metis
-
-(* CFG? *)
-lemma fresh_set: "B \<notin> Nts P \<Longrightarrow> (A,u) \<in> P \<Longrightarrow> Nt B \<notin> set u"
-unfolding Nts_def using nts_syms_set1 by fastforce
-
-(* CFG? *)
-lemma syms_inv:
-  "s \<in> Syms P \<longleftrightarrow> (\<exists>A u. (A,u) \<in> P \<and> (s = Nt A \<or> s \<in> set u))"
-unfolding Syms_def by auto
-
-(* CFG? *)
-lemma syms_subset: 
-  "P \<subseteq> P' \<Longrightarrow> s \<in> Syms P \<Longrightarrow> s \<in> Syms P'"
-unfolding Syms_def by auto
-
-(* CFG? *)
-lemma syms_not_eq: "Nt B \<notin> Syms P \<Longrightarrow> (A,u) \<in> P \<Longrightarrow> A \<noteq> B"
-  using syms_inv by blast
-
-(* CFG? *)
-lemma syms_not_set: "Nt B \<notin> Syms P \<Longrightarrow> (A,u) \<in> P \<Longrightarrow> Nt B \<notin> set u"
-  using syms_inv by blast
-
-(* CFG? *)
-lemma syms_Lhss: "Nt B \<notin> Syms P \<Longrightarrow> B \<notin> Lhss P"
-unfolding Lhss_def Syms_def by auto
-
-(* CFG? *)
-lemma syms_subset2: "Nt B \<notin> Syms P \<Longrightarrow> P' \<subseteq> P \<Longrightarrow> Nt B \<notin> Syms P'"
-  using syms_subset by blast
-
-(* CFG? *)
-lemma syms_set: "a \<notin> Syms P \<Longrightarrow> (A,u) \<in> P \<Longrightarrow> a \<notin> set u"
-  using syms_inv by blast
-
-(* CFG? *)
-lemma fresh_syms: "B \<notin> Nts P \<Longrightarrow> Nt B \<notin> Syms P"
-  by (metis syms_to_Nts)
-
-(* CFG? *)
-lemma syms_Lhss_not_eq: "Nt B \<notin> Syms P \<Longrightarrow> A \<in> Lhss P \<Longrightarrow> A \<noteq> B"
-  using syms_Lhss by force
-
 text 
 \<open>\<open>substW xs y ys\<close> replaces every occurrence of the element \<open>y\<close> with the list of elements \<open>ys\<close> in the given list \<open>xs\<close>\<close>
 
-fun substW :: "'a list \<Rightarrow> 'a \<Rightarrow> 'a list \<Rightarrow> 'a list" where
-  "substW [] _ _ = []"
-| "substW (x#xs) y ys = (if x = y then ys @ substW xs y ys else x # substW xs y ys)"
+definition "substW y ys xs = concat (map (\<lambda>x. if x=y then ys else [x]) xs)"
+
+lemma substW_simps[simp]:
+  "substW y ys[]  = []"
+  "substW y ys (x#xs) = (if x = y then ys @ substW y ys xs else x # substW y ys xs)"
+unfolding substW_def by auto
 
 subsection \<open>Properties of \<open>substW\<close>\<close>
 
-lemma substW_split: "substW (xs @ xs') y ys = substW xs y ys @ substW xs' y ys"
-  by (induction xs) auto
+lemma substW_split: "substW y ys (xs @ xs') = substW y ys xs @ substW y ys xs'"
+unfolding substW_def by auto
 
-lemma substW_skip: "y \<notin> set xs \<Longrightarrow> substW xs y ys = xs"
-  by (induction xs) auto
+lemma substW_skip: "y \<notin> set xs \<Longrightarrow> substW y ys xs = xs"
+unfolding substW_def by (induction xs) auto
 
-lemma substW_len: "length (substW xs y [y']) = length xs"
-  by (induction xs) auto
+lemma substW_len: "length (substW y [y'] xs) = length xs"
+unfolding substW_def by (induction xs) auto
 
-lemma substW_rev: "y' \<notin> set xs \<Longrightarrow> substW (substW xs y [y']) y' [y] = xs"
-  by (induction xs) auto
+lemma substW_rev: "y' \<notin> set xs \<Longrightarrow> substW y' [y] (substW y [y'] xs) = xs"
+unfolding substW_def by (induction xs) auto
 
 lemma substW_der:
-  "(B,v) \<in> P \<Longrightarrow> P \<turnstile> u \<Rightarrow>* substW u (Nt B) v"
+  "(B,v) \<in> P \<Longrightarrow> P \<turnstile> u \<Rightarrow>* substW (Nt B) v u"
+unfolding substW_def
 proof (induction u)
   case Nil
   then show ?case by simp
 next
   case (Cons a u)
   then show ?case
-    by (metis (no_types, lifting) derivel_Nt_Cons derivel_imp_derive derives_Cons rtranclp.rtrancl_into_rtrancl substW.simps(2))
+    by (auto simp add: derives_Cons_rule derives_prepend derives_Cons)
 qed
 
 text
 \<open>\<open>substP ps s u\<close> replaces every occurrence of the symbol \<open>s\<close> with the list of symbols \<open>u\<close> on the right-hand sides of the production list \<open>ps\<close>\<close>
 
-definition substP :: "('n, 't) prods \<Rightarrow>  ('n, 't) sym \<Rightarrow>  ('n, 't) syms \<Rightarrow> ('n, 't) prods" where
-  "substP ps s u = map (\<lambda>(A,v). (A, substW v s u)) ps"
+definition substP :: "('n, 't) sym \<Rightarrow>  ('n, 't) syms \<Rightarrow> ('n, 't) prods \<Rightarrow> ('n, 't) prods" where
+  "substP s u ps = map (\<lambda>(A,v). (A, substW s u v)) ps"
 
 subsection \<open>Properties of \<open>substP\<close>\<close>
 
-lemma substP_split: "substP (ps @ ps') s u = substP ps s u @ substP ps' s u"
+lemma substP_split: "substP s u (ps @ ps') = substP s u ps @ substP s u ps'"
   by (simp add: substP_def)
 
-lemma substP_skip1: "s \<notin> set v \<Longrightarrow> substP ((A,v) # ps) s u = (A,v) # substP ps s u"
+lemma substP_skip1: "s \<notin> set v \<Longrightarrow> substP s u ((A,v) # ps) = (A,v) # substP s u ps"
   by (auto simp add: substW_skip substP_def)
 
-lemma substP_skip2: "s \<notin> syms ps \<Longrightarrow> substP ps s u = ps"
+lemma substP_skip2: "s \<notin> syms ps \<Longrightarrow> substP s u ps = ps"
   by (induction ps) (auto simp add: substP_def substW_skip)
 
-lemma substP_rev: "Nt B \<notin> syms ps \<Longrightarrow> substP (substP ps s [Nt B]) (Nt B) [s] = ps"
+lemma substP_rev: "Nt B \<notin> syms ps \<Longrightarrow> substP (Nt B) [s] (substP s [Nt B] ps) = ps"
 proof (induction ps)
   case Nil
   then show ?case
     by (simp add: substP_def)
 next
   case (Cons a ps)
-  let ?A = "fst a" let ?u = "snd a"
-  have "substP (substP (a # ps) s [Nt B]) (Nt B) [s] = substP (map (\<lambda>(A,v). (A, substW v s [Nt B])) (a#ps)) (Nt B) [s]"
+  let ?A = "fst a" let ?u = "snd a" let ?substs = "substW s [Nt B]"
+  have "substP (Nt B) [s] (substP s [Nt B] (a # ps)) = substP (Nt B) [s] (map (\<lambda>(A,v). (A, ?substs v)) (a#ps))"
     by (simp add: substP_def)
-  also have "... = substP ((?A, substW ?u s [Nt B]) # map (\<lambda>(A,v). (A, substW v s [Nt B])) ps) (Nt B) [s]"
+  also have "... = substP (Nt B) [s] ((?A, ?substs ?u) # map (\<lambda>(A,v). (A, ?substs v)) ps)"
     by (simp add: case_prod_unfold)
-  also have "... = map ((\<lambda>(A,v). (A, substW v (Nt B) [s]))) ((?A, substW ?u s [Nt B]) # map (\<lambda>(A,v). (A, substW v s [Nt B])) ps)"
+  also have "... = map ((\<lambda>(A,v). (A, substW (Nt B) [s] v))) ((?A, ?substs ?u) # map (\<lambda>(A,v). (A, ?substs v)) ps)"
     by (simp add: substP_def)
-  also have "... = (?A, substW (substW ?u s [Nt B]) (Nt B) [s]) # substP (substP ps s [Nt B]) (Nt B) [s]"
+  also have "... = (?A, substW (Nt B) [s] (?substs ?u)) # substP (Nt B) [s] (substP s [Nt B] ps)"
     by (simp add: substP_def)
-  also from Cons have "... = (?A, substW (substW ?u s [Nt B]) (Nt B) [s]) # ps"
-    using syms_subset set_subset_Cons by metis
+  also from Cons have "... = (?A, substW (Nt B) [s] (?substs ?u)) # ps"
+    using set_subset_Cons unfolding Syms_def by auto
   also from Cons.prems have "... = (?A, ?u) # ps"
-    using substW_rev syms_inv by (metis list.set_intros(1) prod.collapse)
+    using substW_rev unfolding Syms_def by force
   also have "... = a # ps" by simp
   finally show ?case .
 qed
 
 lemma substP_lhss:
-  "lhss ps = lhss (substP ps s u)"
+  "lhss ps = lhss (substP s u ps)"
 by (auto simp add: Lhss_def substP_def)
 
 lemma if_set_map:
@@ -184,15 +93,15 @@ lemma if_set_map:
   by auto
 
 lemma substP_der:
-  "(A,u) \<in> set (substP ps (Nt B) v) \<Longrightarrow> set ((B,v) # ps) \<turnstile> [Nt A] \<Rightarrow>* u"
+  "(A,u) \<in> set (substP (Nt B) v ps) \<Longrightarrow> set ((B,v) # ps) \<turnstile> [Nt A] \<Rightarrow>* u"
 proof -
-  assume "(A,u) \<in> set (substP ps (Nt B) v)"
-  then have "\<exists>u'. (A,u') \<in> set ps \<and> u = substW u' (Nt B) v" 
+  assume "(A,u) \<in> set (substP (Nt B) v ps)"
+  then have "\<exists>u'. (A,u') \<in> set ps \<and> u = substW (Nt B) v u'" 
     using if_set_map by (smt (verit, del_insts) Pair_inject case_prod_conv old.prod.exhaust substP_def)
-  then obtain u' where u'_def: "(A,u') \<in> set ps \<and> u = substW u' (Nt B) v" by blast
+  then obtain u' where u'_def: "(A,u') \<in> set ps \<and> u = substW (Nt B) v u'" by blast
   then have path1: "set ((B,v) # ps) \<turnstile> [Nt A] \<Rightarrow>* u'"
     by (simp add: derive_singleton r_into_rtranclp)
-  have "set ((B,v) # ps) \<turnstile> u' \<Rightarrow>* substW u' (Nt B) v"
+  have "set ((B,v) # ps) \<turnstile> u' \<Rightarrow>* substW (Nt B) v u'"
     using substW_der by (metis list.set_intros(1))
   with u'_def have path2: "set ((B,v) # ps) \<turnstile> u' \<Rightarrow>* u" by simp
   from path1 path2 show ?thesis by simp
@@ -204,7 +113,7 @@ text
  \<open>u\<close> can be derived before the procedure, if \<open>u\<close> can be derived after the procedure\<close>
 
 lemma if_part:
-  "set (substP ps (Nt B) v) \<turnstile> [Nt A] \<Rightarrow>* u \<Longrightarrow> set ((B,v) # ps) \<turnstile> [Nt A] \<Rightarrow>* u"
+  "set (substP (Nt B) v ps) \<turnstile> [Nt A] \<Rightarrow>* u \<Longrightarrow> set ((B,v) # ps) \<turnstile> [Nt A] \<Rightarrow>* u"
 proof (induction rule: derives_induct)
   case (step u A v w)
   then show ?case 
@@ -221,7 +130,7 @@ lemma substPW_der:
       and A_B_noteq: "A \<noteq> B"
       and B_notin_dom: "B \<notin> lhss ps"
       and B_notin_v: "Nt B \<notin> set v"
-    shows "set (substP ps (Nt B) v) \<turnstile> [Nt A] \<Rightarrow>* substW u (Nt B) v"
+    shows "set (substP (Nt B) v ps) \<turnstile> [Nt A] \<Rightarrow>* substW (Nt B) v u"
 using assms(1) proof (induction rule: derives_induct)
   case base
   then show ?case using assms(2) by simp
@@ -232,7 +141,7 @@ next
     case True
     then have "v = v'" 
       using B_notin_dom step.hyps unfolding Lhss_def by auto
-    then have "substW (s @ [Nt B'] @ w) (Nt B) v = substW (s @ v' @ w) (Nt B) v" 
+    then have "substW (Nt B) v (s @ [Nt B'] @ w) = substW (Nt B) v (s @ v' @ w)" 
       using step.prems B_notin_v True by (simp add: substW_skip substW_split)
     then show ?thesis
       using step.IH by argo
@@ -240,10 +149,10 @@ next
     case False
     then have "(B',v') \<in> set ps"
       using step by auto
-    then have "(B', substW v' (Nt B) v) \<in> set (substP ps (Nt B) v)"
+    then have "(B', substW (Nt B) v v') \<in> set (substP (Nt B) v ps)"
       by (metis (no_types, lifting) list.set_map pair_imageI substP_def)
-    with rtrancl_into_rtrancl show ?thesis 
-      by (smt (verit, ccfv_threshold) False step.IH step.prems derive.simps rtranclp.simps substW.simps(1) substW.simps(2) substW_split sym.inject(1))
+    with rtrancl_into_rtrancl show ?thesis
+      by (smt (verit, ccfv_threshold) False step.IH step.prems derive.simps rtranclp.simps substW_simps substW_split sym.inject(1))
   qed
 qed
 
@@ -256,7 +165,7 @@ lemma only_if_part:
       and B_notin_dom: "B \<notin> lhss ps"
       and B_notin_v: "Nt B \<notin> set v"
       and B_notin_u: "Nt B \<notin> set u"
-    shows "set (substP ps (Nt B) v) \<turnstile> [Nt A] \<Rightarrow>* u"
+    shows "set (substP (Nt B) v ps) \<turnstile> [Nt A] \<Rightarrow>* u"
   by (metis assms substW_skip substPW_der)
 
 text
@@ -267,7 +176,7 @@ lemma substP_lang:
           "Nt B \<notin> set v" and
           "Nt B \<notin> set u" and
           "A \<noteq> B"
-        shows "set (substP ps (Nt B) v) \<turnstile> [Nt A] \<Rightarrow>* u \<longleftrightarrow> set ((B,v) # ps) \<turnstile> [Nt A] \<Rightarrow>* u"
+        shows "set (substP (Nt B) v ps) \<turnstile> [Nt A] \<Rightarrow>* u \<longleftrightarrow> set ((B,v) # ps) \<turnstile> [Nt A] \<Rightarrow>* u"
   using assms if_part only_if_part by metis
 
 end
